adding used function to smartphone events theory

security-protocols/dap/EventSP.thy
@@ -7,18 +7,17 @@ consts  (*Initial states of agents -- parameter of the construction*)
 
 datatype smartphone = Smarphone agent
 
-text{*Four new events express the traffic between an agent and his card*}
 datatype  
   event = Says  agent agent msg
         | Notes agent       msg
         | Gets  agent       msg
-        | Shows agent smartphone msg
-        | Scans smartphone  msg 
+        | Shows agent       msg
+        | Scans smartphone agent msg 
     
 consts 
- bad     :: "agent set"  (*compromised agents*)
- stolen  :: "smartphone set" (* stolen smart cards *)
- secureM :: "bool"(*assumption of secure means between agents and their cards*)
+ bad     :: "agent set"  (* compromised agents *)
+ stolen  :: "smartphone set" (* stolen smartphones *)
+ secureM :: "bool" (* assumption of secure means between agents and their phones *)
 
 specification (bad)
   Spy_in_bad  [iff]: "Spy \<in> bad"
@@ -32,4 +31,49 @@ specification (stolen)
   apply blast
   done
 
+ 
+primrec used :: "event list \<Rightarrow> msg set" where
+  used_Nil: "used [] = (\<Union> B. parts (initState B))" |
+  used_Cons: 
+    "used (ev # evs) = 
+      (case ev of   
+        Says A B X \<Rightarrow> parts {X} \<union> (used evs) |
+        Notes A X \<Rightarrow> parts {X} \<union> (used evs) |
+        Gets A X \<Rightarrow> used evs |
+        Shows P X \<Rightarrow> parts {X} \<union> (used evs) |
+        Scans P A X \<Rightarrow> parts {X} \<union> (used evs))" 
+
+lemma Notes_imp_used [rule_format]: "Notes A X \<in> set evs --> X \<in> used evs"
+apply (induct_tac evs)
+apply (auto split: event.split) 
+done
+
+lemma Says_imp_used [rule_format]: "Says A B X \<in> set evs --> X \<in> used evs"
+apply (induct_tac evs)
+apply (auto split: event.split) 
+done
+
+lemma MPair_used [rule_format]:
+     "MPair X Y \<in> used evs --> X \<in> used evs & Y \<in> used evs"
+apply (induct_tac evs)
+apply (auto split: event.split) 
+done
+
+
+
+(* primrec knows :: "agent \<Rightarrow> event list \<Rightarrow> msg set" where
+  knows_Nil: "knows A [] = initState A" |
+  knows_Cons: 
+    "knows A (ev # evs) = (case ev of
+      Says A' B X \<Rightarrow>
+        if (A = A' | A = Spy) then insert X (knows A evs) else knows A evs |
+      Notes A' X \<Rightarrow>
+        if (A = A' | (A = Spy & A' \<in> bad)) then insert X (knows A evs) else knows A evs |
+      Gets A' X \<Rightarrow>
+        if (A = A' & A \<noteq> Spy) then insert X (knows A evs) else knows A evs |
+      Shows A' X \<Rightarrow>
+        if (A = A' | A = Spy) then insert X (knows A evs) else knows A evs |
+      Scans P A' X \<Rightarrow> 
+        if () )"
+*)             
 end
